src/HOL/Lambda/ListApplication.thy
@@ -9,26 +9,23 @@ header {* Application of a term to a list of terms *}
 theory ListApplication = Lambda:
 
 syntax
-  "_list_application" :: "dB => dB list => dB"    (infixl "$$" 150)
-syntax (symbols)
-  "_list_application" :: "dB => dB list => dB"    (infixl "\<^sub>\<degree>\<^sub>\<degree>" 150)
-
+  "_list_application" :: "dB => dB list => dB"    (infixl "\<degree>\<degree>" 150)
 translations
-  "t $$ ts" == "foldl (op $) t ts"
+  "t \<degree>\<degree> ts" == "foldl (op \<degree>) t ts"
 
-lemma apps_eq_tail_conv [iff]: "(r $$ ts = s $$ ts) = (r = s)"
+lemma apps_eq_tail_conv [iff]: "(r \<degree>\<degree> ts = s \<degree>\<degree> ts) = (r = s)"
   apply (induct_tac ts rule: rev_induct)
    apply auto
   done
 
 lemma Var_eq_apps_conv [rule_format, iff]:
-    "\<forall>s. (Var m = s $$ ss) = (Var m = s \<and> ss = [])"
+    "\<forall>s. (Var m = s \<degree>\<degree> ss) = (Var m = s \<and> ss = [])"
   apply (induct_tac ss)
    apply auto
   done
 
 lemma Var_apps_eq_Var_apps_conv [rule_format, iff]:
-    "\<forall>ss. (Var m $$ rs = Var n $$ ss) = (m = n \<and> rs = ss)"
+    "\<forall>ss. (Var m \<degree>\<degree> rs = Var n \<degree>\<degree> ss) = (m = n \<and> rs = ss)"
   apply (induct_tac rs rule: rev_induct)
    apply simp
    apply blast
@@ -38,26 +35,26 @@ lemma Var_apps_eq_Var_apps_conv [rule_format, iff]:
   done
 
 lemma App_eq_foldl_conv:
-  "(r $ s = t $$ ts) =
-    (if ts = [] then r $ s = t
-    else (\<exists>ss. ts = ss @ [s] \<and> r = t $$ ss))"
+  "(r \<degree> s = t \<degree>\<degree> ts) =
+    (if ts = [] then r \<degree> s = t
+    else (\<exists>ss. ts = ss @ [s] \<and> r = t \<degree>\<degree> ss))"
   apply (rule_tac xs = ts in rev_exhaust)
    apply auto
   done
 
 lemma Abs_eq_apps_conv [iff]:
-    "(Abs r = s $$ ss) = (Abs r = s \<and> ss = [])"
+    "(Abs r = s \<degree>\<degree> ss) = (Abs r = s \<and> ss = [])"
   apply (induct_tac ss rule: rev_induct)
    apply auto
   done
 
-lemma apps_eq_Abs_conv [iff]: "(s $$ ss = Abs r) = (s = Abs r \<and> ss = [])"
+lemma apps_eq_Abs_conv [iff]: "(s \<degree>\<degree> ss = Abs r) = (s = Abs r \<and> ss = [])"
   apply (induct_tac ss rule: rev_induct)
    apply auto
   done
 
 lemma Abs_apps_eq_Abs_apps_conv [iff]:
-    "\<forall>ss. (Abs r $$ rs = Abs s $$ ss) = (r = s \<and> rs = ss)"
+    "\<forall>ss. (Abs r \<degree>\<degree> rs = Abs s \<degree>\<degree> ss) = (r = s \<and> rs = ss)"
   apply (induct_tac rs rule: rev_induct)
    apply simp
    apply blast
@@ -67,13 +64,13 @@ lemma Abs_apps_eq_Abs_apps_conv [iff]:
   done
 
 lemma Abs_App_neq_Var_apps [iff]:
-    "\<forall>s t. Abs s $ t ~= Var n $$ ss"
+    "\<forall>s t. Abs s \<degree> t ~= Var n \<degree>\<degree> ss"
   apply (induct_tac ss rule: rev_induct)
    apply auto
   done
 
 lemma Var_apps_neq_Abs_apps [rule_format, iff]:
-    "\<forall>ts. Var n $$ ts ~= Abs r $$ ss"
+    "\<forall>ts. Var n \<degree>\<degree> ts ~= Abs r \<degree>\<degree> ss"
   apply (induct_tac ss rule: rev_induct)
    apply simp
   apply (rule allI)
@@ -82,19 +79,19 @@ lemma Var_apps_neq_Abs_apps [rule_format, iff]:
   done
 
 lemma ex_head_tail:
-  "\<exists>ts h. t = h $$ ts \<and> ((\<exists>n. h = Var n) \<or> (\<exists>u. h = Abs u))"
+  "\<exists>ts h. t = h \<degree>\<degree> ts \<and> ((\<exists>n. h = Var n) \<or> (\<exists>u. h = Abs u))"
   apply (induct_tac t)
     apply (rule_tac x = "[]" in exI)
     apply simp
    apply clarify
    apply (rename_tac ts1 ts2 h1 h2)
-   apply (rule_tac x = "ts1 @ [h2 $$ ts2]" in exI)
+   apply (rule_tac x = "ts1 @ [h2 \<degree>\<degree> ts2]" in exI)
    apply simp
   apply simp
   done
 
 lemma size_apps [simp]:
-  "size (r $$ rs) = size r + foldl (op +) 0 (map size rs) + length rs"
+  "size (r \<degree>\<degree> rs) = size r + foldl (op +) 0 (map size rs) + length rs"
   apply (induct_tac rs rule: rev_induct)
    apply auto
   done
@@ -104,11 +101,11 @@ lemma lem0: "[| (0::nat) < k; m <= n |] ==> m < n + k"
   done
 
 
-text {* \medskip A customized induction schema for @{text "$$"}. *}
+text {* \medskip A customized induction schema for @{text "\<degree>\<degree>"}. *}
 
 lemma lem [rule_format (no_asm)]:
-  "[| !!n ts. \<forall>t \<in> set ts. P t ==> P (Var n $$ ts);
-    !!u ts. [| P u; \<forall>t \<in> set ts. P t |] ==> P (Abs u $$ ts)
+  "[| !!n ts. \<forall>t \<in> set ts. P t ==> P (Var n \<degree>\<degree> ts);
+    !!u ts. [| P u; \<forall>t \<in> set ts. P t |] ==> P (Abs u \<degree>\<degree> ts)
   |] ==> \<forall>t. size t = n --> P t"
 proof -
   case rule_context
@@ -149,8 +146,8 @@ proof -
 qed
 
 theorem Apps_dB_induct:
-  "[| !!n ts. \<forall>t \<in> set ts. P t ==> P (Var n $$ ts);
-    !!u ts. [| P u; \<forall>t \<in> set ts. P t |] ==> P (Abs u $$ ts)
+  "[| !!n ts. \<forall>t \<in> set ts. P t ==> P (Var n \<degree>\<degree> ts);
+    !!u ts. [| P u; \<forall>t \<in> set ts. P t |] ==> P (Abs u \<degree>\<degree> ts)
   |] ==> P t"
 proof -
   case rule_context
